update monotone references

src/mono_ref.v
@@ -13,60 +13,37 @@ Section Resources.
 
   Class MonRefG Σ := monrefG {
     MonRefIG_monauth :> inG Σ (authUR (monotoneUR R));
-    MonRefIG_register :> inG Σ (authUR (gmapUR loc (agreeR (leibnizC gname))));
-    MonRefIG_register_name : gname;
-  }.
-
-  Class MonRefPreG Σ := monrefPreG {
-    MonRefPreIG_monauth :> inG Σ (authUR (monotoneUR R));
-    MonRefPreIG_register :> inG Σ (authUR (gmapUR loc (agreeR (leibnizC gname))));
   }.
 
   Definition MonRefΣ :=
-    #[GFunctor (authUR (monotoneUR R));
-        GFunctor (authUR (gmapUR loc (agreeR (leibnizC gname))))].
+    #[GFunctor (authUR (monotoneUR R))].
 
-  Instance subG_MonRefIGΣ {Σ} : subG MonRefΣ Σ → MonRefPreG Σ.
+  Instance subG_MonRefIGΣ {Σ} : subG MonRefΣ Σ → MonRefG Σ.
   Proof. solve_inG. Qed.
 End Resources.
 
 Global Arguments MonRefG {_} _ _.
-Global Arguments MonRefPreG {_} _ _.
 
 Section MonRef.
   Context {A : ofeT} (R : relation A) `{!ProperPreOrder R}.
   Context (to_A : val → option A).
   Context `{!MonRefG R Σ, !heapG Σ}.
 
-  Definition MonRefN := nroot .@ "MonoRef".
-
-  Definition toRegister (M : gmap loc gname) :
-    gmapUR loc (agreeR (leibnizC gname)) := (λ x, to_agree x) <$> M.
-
-  Definition LocRegister M := own MonRefIG_register_name (● toRegister M).
-  Definition registered l (γ : gname) :=
-    own MonRefIG_register_name (◯ {[l := to_agree γ]}).
-
-  Lemma registered_agree l γ γ' : registered l γ -∗ registered l γ' -∗ ⌜γ = γ'⌝.
-  Proof.
-    iIntros "H1 H2".
-    iDestruct (own_valid_2 with "H1 H2") as %Hvl.
-    iPureIntro.
-    specialize (Hvl l); revert Hvl;
-      rewrite /= lookup_op !lookup_singleton -Some_op Some_valid.
-      intros Hvl%@agree_op_inv'; eauto.
-  Qed.
-
-  Definition MonRefFull γ v :=
+  Definition Exact γ v :=
     (∃ a, ⌜to_A v = Some a⌝ ∗ own γ (● (principal R a)))%I.
 
-  Definition MonRefFrag γ v :=
+  Definition atleast_def γ v :=
     (∃ a, ⌜to_A v = Some a⌝ ∗ own γ (◯ (principal R a)))%I.
+  Definition atleast_aux γ v : seal (atleast_def γ v). by eexists. Qed.
+  Definition atleast γ v : iProp Σ := (atleast_aux γ v).(unseal).
+  Definition atleast_eq γ v : atleast γ v = atleast_def γ v :=
+    (atleast_aux γ v).(seal_eq).
 
   Lemma MonRef_related γ v w :
-    MonRefFull γ v -∗ MonRefFrag γ w -∗
+    Exact γ v -∗ atleast γ w -∗
                ∃ a b, ⌜to_A w = Some a ∧ to_A v = Some b ∧ R a b⌝.
   Proof.
+    rewrite atleast_eq /atleast_def.
     iIntros "HF Hf".
     iDestruct "HF" as (a ->) "HF".
     iDestruct "Hf" as (b ->) "Hf".
@@ -76,73 +53,34 @@ Section MonRef.
     rewrite left_id_L in Hvl. apply (principal_included b a) in Hvl; eauto.
   Qed.
 
-  Definition atleast_def l v := (∃ γ, registered l γ ∗ MonRefFrag γ v)%I.
-  Definition atleast_aux l v : seal (atleast_def l v). by eexists. Qed.
-  Definition atleast l v : iProp Σ := (atleast_aux l v).(unseal).
-  Definition atleast_eq l v : atleast l v = atleast_def l v :=
-    (atleast_aux l v).(seal_eq).
-
   Global Instance atleas_presistent l v : Persistent (atleast l v).
   Proof. rewrite atleast_eq /atleast_def; apply _. Qed.
 
-  Definition MonRefInv_body :=
-    (∃ M, LocRegister M ∗ [∗ set] l ∈ (dom (gset _) M), l ↦{1/2} -)%I.
-
-  Definition MonRefInv : iProp Σ := inv MonRefN MonRefInv_body.
-
-  Definition MonRefMapsto_def l q v :=
-    (MonRefInv ∗ ∃ γ, registered l γ ∗ MonRefFull γ v
-                                 ∗ MonRefFrag γ v ∗ l ↦{q /2} v)%I.
-  Definition MonRefMapsto_aux l q v : seal (MonRefMapsto_def l q v).
+  Definition MonRefMapsto_def l γ q v :=
+    (Exact γ v ∗ atleast γ v ∗ l ↦{q} v)%I.
+  Definition MonRefMapsto_aux l γ q v : seal (MonRefMapsto_def l γ q v).
   Proof. by eexists. Qed.
-  Definition MonRefMapsto l q v : iProp Σ := (MonRefMapsto_aux l q v).(unseal).
-  Definition MonRefMapsto_eq l q v :
-    MonRefMapsto l q v = MonRefMapsto_def l q v :=
-    (MonRefMapsto_aux l q v).(seal_eq).
+  Definition MonRefMapsto l γ q v : iProp Σ := (MonRefMapsto_aux l γ q v).(unseal).
+  Definition MonRefMapsto_eq l γ q v :
+    MonRefMapsto l γ q v = MonRefMapsto_def l γ q v :=
+    (MonRefMapsto_aux l γ q v).(seal_eq).
 
-  Lemma lookup_register M l γ :
-    LocRegister M -∗ registered l γ -∗ ⌜M !! l = Some γ⌝.
+  Lemma MonRef_alloc v a :
+    to_A v = Some a → (|==> ∃ γ, Exact γ v ∗ atleast γ v)%I.
   Proof.
-    iIntros "Hlv HM".
-    iDestruct (own_valid_2 with "Hlv HM") as %[Hv HMv]; simpl in *.
-      iPureIntro.
-      specialize (Hv O); apply cmra_discrete_included_iff in Hv.
-      destruct Hv as [z Hv]; specialize (Hv l). specialize (HMv l).
-      revert Hv HMv. rewrite left_id /toRegister lookup_fmap lookup_op.
-      intros Hv; rewrite Hv.
-      intros HMv. pose proof (cmra_valid_op_r _ _ HMv) as HMv'.
-      revert Hv HMv HMv'. case: (z !! l).
-      - intros a Hv HMv HMv'.
-        destruct (to_agree_uninj _ HMv') as [? Heq].
-        revert HMv Hv. rewrite -Heq lookup_singleton; intros HMv Hv.
-        apply agree_op_invL' in HMv; subst.
-        revert Hv. rewrite -Some_op agree_idemp.
-        case (M !! l); simpl; last by inversion 1.
-        intros ? HMv.
-        by apply Some_equiv_inj, @to_agree_inj, leibniz_equiv in HMv; subst.
-      - rewrite right_id lookup_singleton.
-        case (M !! l); simpl; last by inversion 1.
-        intros ? HMv.
-        by apply Some_equiv_inj, @to_agree_inj, leibniz_equiv in HMv; subst.
-  Qed.
-
-  Lemma MonRefInv_body_lookup l γ :
-    registered l γ -∗ MonRefInv_body -∗
-      l ↦{1/2} - ∗ ((l ↦{1/2} -) -∗ MonRefInv_body).
-  Proof.
-    iIntros "#Hlv Hbd"; iDestruct "Hbd" as (M) "[HM Hreg]".
-    iDestruct (lookup_register with "HM Hlv") as %?.
-    rewrite (big_sepS_elem_of_acc _ _ l); last by apply elem_of_dom; eauto.
-    iDestruct "Hreg" as "[$ Hreg]".
-    iIntros "Hl".
-    iExists _; iFrame.
-    by iApply "Hreg".
+    setoid_rewrite atleast_eq. rewrite /atleast_def /Exact.
+    iIntros (Hv).
+    iMod (own_alloc (● (principal R a) ⋅ ◯ (principal R a))) as (γ) "[HF Hf]".
+    { rewrite auth_valid_eq /=; split; last done. intros ?; rewrite left_id.
+      by eapply (principal_includedN). }
+    iModIntro; iExists _; iSplitL "HF"; iFrame; eauto.
   Qed.
 
   Lemma MonRef_update γ v w a b :
     to_A v = Some a → to_A w = Some b → R a b →
-    MonRefFull γ v ==∗ MonRefFull γ w ∗ MonRefFrag γ w.
+    Exact γ v ==∗ Exact γ w ∗ atleast γ w.
   Proof.
+    rewrite atleast_eq /atleast_def.
     iIntros (Hv Hw HR) "HF".
     iDestruct "HF" as (c Hc) "HF"; simplify_eq.
     iMod (own_update _ _ (● (principal R b) ⋅ ◯ (principal R b))
@@ -154,126 +92,69 @@ Section MonRef.
     iModIntro; iSplitL "HF"; iExists _; iSplit; eauto.
   Qed.
 
-  Lemma Register_loc l v a M :
-    to_A v = Some a → M !! l = None →
-    LocRegister M ==∗ ∃ γ, LocRegister (<[l := γ ]>M) ∗ registered l γ ∗
-                           MonRefFull γ v ∗ MonRefFrag γ v.
+  Lemma MonRefAlloc l v a :
+    to_A v = Some a → l ↦ v ==∗ ∃ γ, MonRefMapsto l γ 1 v.
   Proof.
-    iIntros (Hv Hl) "HM".
-    iMod (own_alloc (● (principal R a) ⋅ (◯ (principal R a))))
-      as (γ) "[HFl HFr]"; first done.
-    iMod (own_update _ _ (● toRegister (<[l := γ ]>M) ⋅ ◯ {[l := to_agree γ]})
-            with "HM") as "[HM Hreg]".
-    { apply auth_update_alloc. rewrite /toRegister fmap_insert.
-      apply @alloc_singleton_local_update; last done.
-      by rewrite lookup_fmap Hl. }
-    iModIntro; iExists _; iFrame.
-    by iSplit; iExists _; iFrame.
-  Qed.
-
-  Lemma MonRefAlloc E l v a :
-    nclose MonRefN ⊆ E → to_A v = Some a →
-    MonRefInv -∗ l ↦ v ={E}=∗ MonRefMapsto l 1 v.
-  Proof.
-    iIntros (HE Hv) "#Hinv Hl".
-    iInv MonRefN as (M) ">[HM Hpts]" "Hcl".
-    iAssert (⌜M !! l = None⌝)%I with "[Hl Hpts]" as %?.
-    { destruct (M !! l) as [x|] eqn:Hx; auto.
-      iDestruct (big_sepS_elem_of_acc  _ _ l with "Hpts") as "[Hpt _]";
-        first by apply elem_of_dom; eauto.
-      iDestruct "Hpt" as (w) "[Hpt _]".
-      by iDestruct (@mapsto_valid_2 with "Hl Hpt") as "%". }
-    iMod (Register_loc with "HM") as (γ) "(HM & Hreg & HFl & HFr)"; eauto.
-    iDestruct "Hl" as "[Hl1 Hl2]".
-    iMod ("Hcl" with "[HM Hpts Hl1]") as "_".
-    { iNext. iExists _; iFrame "HM".
-      rewrite dom_insert_L big_sepS_insert; last by apply not_elem_of_dom.
-      iFrame; eauto. }
-    iModIntro.
-    rewrite MonRefMapsto_eq /MonRefMapsto_def. iFrame "#"; iExists _; iFrame.
+    iIntros (Hv) "Hl".
+    iMod (MonRef_alloc v a) as (γ) "[HE Hal]"; eauto.
+    iModIntro. iExists _.
+    rewrite MonRefMapsto_eq /MonRefMapsto_def. iFrame.
   Qed.
 
   Lemma wp_Create_MonRef E (v : val) :
-    nclose MonRefN ⊆ E →
-    {{{ MonRefInv ∗ ∃ a, ⌜to_A v = Some a⌝ }}}
+    {{{ ∃ a, ⌜to_A v = Some a⌝ }}}
       Alloc v @ E
-    {{{l, RET (Lit $ LitLoc l); MonRefMapsto l 1 v }}}.
+    {{{l γ, RET (Lit $ LitLoc l); MonRefMapsto l γ 1 v }}}.
   Proof.
-    iIntros (HE F) "[#HI H] HF". iDestruct "H" as (a) "%".
+    iIntros (F) "H HF". iDestruct "H" as (a) "%".
     iApply wp_fupd.
     wp_alloc l as "Hl".
-    iMod (MonRefAlloc with "[] Hl"); eauto.
+    iMod (MonRefAlloc with "Hl") as (γ) "H"; eauto.
     by iModIntro; iApply "HF".
   Qed.
 
-  Lemma wp_Read_MonRef E l q (v : val) :
-    nclose MonRefN ⊆ E →
-    {{{ MonRefMapsto l q v }}}
+  Lemma wp_Read_MonRef E l γ q (v : val) :
+    {{{ MonRefMapsto l γ q v }}}
       ! (Lit $ LitLoc l) @ E
-    {{{RET v; MonRefMapsto l q v }}}.
+    {{{RET v; MonRefMapsto l γ q v }}}.
   Proof.
     rewrite MonRefMapsto_eq /MonRefMapsto_def.
-    iIntros (HE F) "[#HI H] HF". iDestruct "H" as (γ) "(Hrg & HFl & HFr & Hl)".
+    iIntros (F) "H HF".
+    iDestruct "H" as "(HE & Hal & Hl)".
     wp_load.
-    iApply "HF"; iFrame "#"; iExists _; iFrame.
+    iApply "HF"; iFrame "#"; iFrame.
   Qed.
 
-  Lemma wp_Write_MonRef E l (v w : val) a b :
-    nclose MonRefN ⊆ E →
+  Lemma wp_Write_MonRef E l γ (v w : val) a b :
     to_A v = Some a → to_A w = Some b → R a b →
-    {{{ MonRefMapsto l 1 v }}}
+    {{{ MonRefMapsto l γ 1 v }}}
       (Lit $ LitLoc l) <- w @ E
-    {{{RET #(); MonRefMapsto l 1 w }}}.
+    {{{RET #(); MonRefMapsto l γ 1 w }}}.
   Proof.
     rewrite MonRefMapsto_eq /MonRefMapsto_def.
-    iIntros (HE Hv Hw HR F) "[#HI H] HF".
-    iDestruct "H" as (γ) "(#Hrg & HFl & HFr& Hl)".
-    iInv MonRefN as ">HM" "Hcl".
-    iDestruct (MonRefInv_body_lookup with "Hrg HM") as "[Hlv HM]".
-    iDestruct "Hlv" as (u) "Hlv".
-    iDestruct (@mapsto_agree with "Hl Hlv") as %->.
-    iCombine "Hl" "Hlv" as "Hl".
+    iIntros (Hv Hw HR F) "H HF".
+    iDestruct "H" as "(HE & Hal & Hl)".
+    iApply wp_fupd.
     wp_store.
     iDestruct "Hl" as "[Hl Hl']".
-    iMod (MonRef_update with "HFl") as "[HFl HFr']"; eauto.
-    iMod ("Hcl" with "[HM Hl']") as "_".
-    { iNext. iApply "HM". iExists _; iFrame. }
+    iMod (MonRef_update with "HE") as "[HE HFr']"; eauto.
     iModIntro. iApply "HF".
-    rewrite MonRefMapsto_eq /MonRefMapsto_def; iFrame "#".
-    iExists _; iFrame "#"; iFrame.
+    rewrite MonRefMapsto_eq /MonRefMapsto_def; iFrame.
   Qed.
 
-  Lemma snap_shot l q v : MonRefMapsto l q v -∗ atleast l v.
+  Lemma snap_shot l γ q v : MonRefMapsto l γ q v ==∗ atleast γ v.
   Proof.
     rewrite MonRefMapsto_eq /MonRefMapsto_def atleast_eq /atleast_def.
-    iIntros "[#Hinv Hpt]".
-    iDestruct "Hpt" as (γ) "(?&?&?&?)"; iExists _; iFrame.
+    iIntros "(HE & Hal & Hl)"; eauto.
   Qed.
 
-  Lemma recall l q v w :
-    atleast l w -∗ MonRefMapsto l q v -∗
+  Lemma recall l γ q v w :
+    atleast γ w -∗ MonRefMapsto l γ q v -∗
             ∃ a b, ⌜to_A w = Some a ∧ to_A v = Some b ∧ R a b⌝.
   Proof.
-    rewrite MonRefMapsto_eq /MonRefMapsto_def atleast_eq /atleast_def.
-    iIntros "Hal [#Hinv Hpt]".
-    iDestruct "Hpt" as (γ) "(#Hrg1&HFl&HFr&?)".
-    iDestruct "Hal" as (γ') "(#Hrg2&HFr')".
-    iDestruct (registered_agree with "Hrg1 Hrg2") as %->.
-    iApply (MonRef_related with "HFl HFr'").
+    rewrite MonRefMapsto_eq /MonRefMapsto_def.
+    iIntros "Hal (HE & Hal' & Hl)".
+    iDestruct (MonRef_related with "HE Hal") as "?"; eauto.
   Qed.
 
 End MonRef.
-
-Lemma MonRefG_alloc E {A : ofeT} {R : relation A} `{!ProperPreOrder R}
-      `{!heapG Σ, !MonRefPreG R Σ} :
-  (|={E}=> ∃ _ : MonRefG R Σ, MonRefInv R)%I.
-Proof.
-  iIntros "".
-  iMod (own_alloc (A := (authUR (gmapUR loc (agreeR (leibnizC gname)))))
-                  (● ∅)) as (γ) "?"; first done.
-  iMod (inv_alloc _ _ with "[-]") as "?";
-    last by iExists {| MonRefIG_register_name := γ |}; iFrame.
-  iNext. iExists ∅.
-  rewrite /MonRefInv /MonRefInv_body /LocRegister /toRegister.
-  rewrite fmap_empty dom_empty_L big_sepS_empty; iFrame.
-Qed.
